thys/CoreC++/ClassRel.thy
@@ -1,5 +1,5 @@
 (*  Title:       CoreC++
-    ID:          $Id: ClassRel.thy,v 1.7 2007-02-07 17:24:54 stefanberghofer Exp $
+    ID:          $Id: ClassRel.thy,v 1.8 2007-07-11 10:07:48 stefanberghofer Exp $
     Author:      Daniel Wasserrab
     Maintainer:  Daniel Wasserrab <wasserra at fmi.uni-passau.de>
 
@@ -13,32 +13,35 @@ theory ClassRel imports Decl begin
 
 
 -- "direct repeated subclass"
-inductive2
-  subclsR   :: "prog \<Rightarrow> [cname, cname] \<Rightarrow> bool" ("_ \<turnstile> _ \<prec>\<^sub>R _" [71,71,71] 70)
+inductive_set
+  subclsR :: "prog \<Rightarrow> (cname \<times> cname) set"
+  and subclsR' :: "prog \<Rightarrow> [cname, cname] \<Rightarrow> bool" ("_ \<turnstile> _ \<prec>\<^sub>R _" [71,71,71] 70)
   for P :: prog
 where
-  subclsRI: "\<lbrakk>class P C = Some (Bs,rest); Repeats(D) \<in> set Bs\<rbrakk> 
-\<Longrightarrow> P \<turnstile> C \<prec>\<^sub>R D"
+  "P \<turnstile> C \<prec>\<^sub>R D \<equiv> (C,D) \<in> subclsR P"
+| subclsRI: "\<lbrakk>class P C = Some (Bs,rest); Repeats(D) \<in> set Bs\<rbrakk> \<Longrightarrow> P \<turnstile> C \<prec>\<^sub>R D"
 
 -- "direct shared subclass"
-inductive2
-  subclsS   :: "prog \<Rightarrow> [cname, cname] \<Rightarrow> bool" ("_ \<turnstile> _ \<prec>\<^sub>S _" [71,71,71] 70)
+inductive_set
+  subclsS :: "prog \<Rightarrow> (cname \<times> cname) set"
+  and subclsS' :: "prog \<Rightarrow> [cname, cname] \<Rightarrow> bool" ("_ \<turnstile> _ \<prec>\<^sub>S _" [71,71,71] 70)
   for P :: prog
 where
-  subclsSI: "\<lbrakk>class P C = Some (Bs,rest); Shares(D) \<in> set Bs\<rbrakk> 
-\<Longrightarrow> P \<turnstile> C \<prec>\<^sub>S D"
+  "P \<turnstile> C \<prec>\<^sub>S D \<equiv> (C,D) \<in> subclsS P"
+| subclsSI: "\<lbrakk>class P C = Some (Bs,rest); Shares(D) \<in> set Bs\<rbrakk> \<Longrightarrow> P \<turnstile> C \<prec>\<^sub>S D"
 
  -- "direct subclass"
-inductive2
-  subcls1   :: "prog \<Rightarrow> [cname, cname] \<Rightarrow> bool" ("_ \<turnstile> _ \<prec>\<^sup>1 _" [71,71,71] 70)
+inductive_set
+  subcls1 :: "prog \<Rightarrow> (cname \<times> cname) set"
+  and subcls1' :: "prog \<Rightarrow> [cname, cname] \<Rightarrow> bool" ("_ \<turnstile> _ \<prec>\<^sup>1 _" [71,71,71] 70)
   for P :: prog
 where
-  subcls1I: "\<lbrakk>class P C = Some (Bs,rest); D \<in>  baseClasses Bs\<rbrakk> 
-\<Longrightarrow> P \<turnstile> C \<prec>\<^sup>1 D"
+  "P \<turnstile> C \<prec>\<^sup>1 D \<equiv> (C,D) \<in> subcls1 P"
+| subcls1I: "\<lbrakk>class P C = Some (Bs,rest); D \<in>  baseClasses Bs\<rbrakk> \<Longrightarrow> P \<turnstile> C \<prec>\<^sup>1 D"
 
 abbreviation
   subcls    :: "prog \<Rightarrow> [cname, cname] \<Rightarrow> bool" ("_ \<turnstile> _ \<preceq>\<^sup>* _"  [71,71,71] 70) where
-  "P \<turnstile> C \<preceq>\<^sup>* D \<equiv> (subcls1 P)\<^sup>*\<^sup>* C D"
+  "P \<turnstile> C \<preceq>\<^sup>* D \<equiv> (C,D) \<in> (subcls1 P)\<^sup>*"
  
 
 lemma subclsRD:
@@ -67,9 +70,9 @@ lemma subcls1_subclsR_or_subclsS:
 by (auto dest!:subcls1D intro:subclsRI 
   dest:baseClasses_repeats_or_shares subclsSI)
 
-lemma finite_subcls1: "finite (Collect2 (subcls1 P))"
+lemma finite_subcls1: "finite (subcls1 P)"
 
-apply(subgoal_tac "Collect2 (subcls1 P) = (SIGMA C: {C. is_class P C} . 
+apply(subgoal_tac "subcls1 P = (SIGMA C: {C. is_class P C} . 
                      {D. D \<in> baseClasses (fst(the(class P C)))})")
  prefer 2
  apply(fastsimp simp:is_class_def dest: subcls1D elim: subcls1I)
@@ -80,12 +83,12 @@ apply (auto intro:finite_baseClasses simp:is_class_def)
 done
 
 
-lemma finite_subclsR: "finite (Collect2 (subclsR P))"
-by(rule_tac B = "Collect2 (subcls1 P)" in finite_subset, 
+lemma finite_subclsR: "finite (subclsR P)"
+by(rule_tac B = "subcls1 P" in finite_subset, 
   auto simp:subclsR_subcls1 finite_subcls1)
 
-lemma finite_subclsS: "finite (Collect2 (subclsS P))"
-by(rule_tac B = "Collect2 (subcls1 P)" in finite_subset, 
+lemma finite_subclsS: "finite (subclsS P)"
+by(rule_tac B = "subcls1 P" in finite_subset, 
   auto simp:subclsS_subcls1 finite_subcls1)
 
 lemma subcls1_class:
@@ -94,6 +97,6 @@ by (auto dest:subcls1D simp:is_class_def)
 
 lemma subcls_is_class:
 "\<lbrakk>P \<turnstile> D \<preceq>\<^sup>* C; is_class P C\<rbrakk> \<Longrightarrow> is_class P D"
-by (induct rule:rtrancl_induct',auto dest:subcls1_class)
+by (induct rule:rtrancl_induct,auto dest:subcls1_class)
 
 end
